DY/Actions/Random.lean
@@ -148,7 +148,7 @@ public
 abbrev invariants: Bytes.PartialInvariants SubF := Random.Random.invariants
 
 public
-def Random.invariantsProofs [BytesInvariants]: Bytes.PartialInvariantsProofs Random.invariants where
+theorem Random.invariantsProofs [BytesInvariants]: Bytes.PartialInvariantsProofs Random.invariants where
   usage_later := by
     intro x rec tr1 tr2
     simp only [invariants]
