DY/EquationalTheory/DiffieHellman.lean
@@ -203,8 +203,10 @@ end AttackerKnowledge
 
 section Invariants
 
+section Definition
+
 variable [ExecTraceTypes] [ProofTraceTypes]
-variable [BytesFunctor] [BytesFunctor.Has DiffieHellman.SubF]
+variable [BytesFunctor]
 
 public
 def DhPk.invariants: Bytes.PartialInvariants DhPk.SubF where
@@ -221,10 +223,14 @@ def DhPk.invariants: Bytes.PartialInvariants DhPk.SubF where
     (rec sk) tr
 
 public
-def DhPk.invariantsProofs [BytesInvariants]: Bytes.PartialInvariantsProofs DhPk.invariants where
+theorem DhPk.invariantsProofs [BytesInvariants]: Bytes.PartialInvariantsProofs DhPk.invariants where
+
+end Definition
 
 section DhPkLemmas
 
+variable [ExecTraceTypes] [ProofTraceTypes]
+variable [BytesFunctor] [BytesFunctor.Has DiffieHellman.SubF]
 variable [BytesInvariants] [BytesInvariants.Has DhPk.invariants]
 
 @[simp]
@@ -256,6 +262,11 @@ theorem dh_pk.Invariant
 
 end DhPkLemmas
 
+section Definition
+
+variable [ExecTraceTypes] [ProofTraceTypes]
+variable [BytesFunctor] [BytesFunctor.Has DiffieHellman.SubF]
+
 public
 def Dh.invariants: Bytes.PartialInvariants Dh.SubF where
   well_formed := fun {pk, sk} rec tr =>
@@ -276,11 +287,13 @@ def Dh.invariants: Bytes.PartialInvariants Dh.SubF where
       (rec sk) tr
 
 public
-def Dh.invariantsProofs [BytesInvariants] [BytesInvariants.Has DhPk.invariants]: Bytes.PartialInvariantsProofs Dh.invariants where
+theorem Dh.invariantsProofs [BytesInvariants] [BytesInvariants.Has DhPk.invariants]: Bytes.PartialInvariantsProofs Dh.invariants where
   label_later := by
     intro _ x rec tr1 tr2
     cases x
     simp_all [DhPk.invariants, invariants, DY.ALaCarte.FunctorSizeOf.sizeOf, GetLabelLaterT] <;> grind
+
+end Definition
 
 #combine [BytesFunctor.Has SubF] into
   BytesInvariants,
